BridgeDefinition/More_Mapping.thy
@@ -26,6 +26,10 @@ lemma lookupNat_delete' [simp]:
   unfolding lookupNat_def
   by (simp add: lookup_default_def)
 
+lemma lookupNat_empty [simp]:
+  shows "lookupNat Mapping.empty x = 0"
+  by (simp add: lookupNat_def lookup_default_empty)
+
 lemma lookupBool_update [simp]: 
   shows "lookupBool (Mapping.update k v m) k = v"
   unfolding lookupBool_def
@@ -55,5 +59,26 @@ lemma mapping_value_sum_update_minus [simp]:
      "mapping_value_sum (Mapping.update k (lookupNat m k - v) m) = mapping_value_sum m - v"
   using assms
   sorry
+
+lemma mapping_value_sum_geq_entry:
+  assumes "finite (Mapping.keys M)" "user \<in> Mapping.keys M"
+  shows "lookupNat M user \<le> mapping_value_sum M"
+proof-
+  have "finite (Mapping.entries M)"
+    using assms
+    by simp
+  moreover
+  have "(user, lookupNat M user) \<in> Mapping.entries M"
+    using assms unfolding lookupNat_def
+    by (metis default_def in_entriesI lookup_default)
+  ultimately
+  have "(user, lookupNat M user) \<in> set (Mapping.ordered_entries M)"
+    using assms
+    unfolding Mapping.ordered_entries_def
+    by (metis (full_types) ordered_entries_def set_ordered_entries)
+  then show ?thesis
+    unfolding mapping_value_sum_def
+    by (metis member_le_sum_list set_zip_rightD zip_map_fst_snd)
+qed
 
 end
